WIP Bring VerilogEquivalence back to speed

vera/VerilogEquivalence.v
@@ -35,9 +35,9 @@ Import FunctorNotation.
 Local Open Scope monad_scope.
 Local Open Scope string.
 
-Equations mk_var_same (var : Verilog.variable) (namemap : VerilogSMTBijection.t)
+Equations mk_var_same (var : Verilog.variable) (m : VerilogSMTBijection.t)
   : sum string SMTLib.term := {
-  | var, namemap with namemap (TaggedVariable.VerilogLeft, var), namemap (TaggedVariable.VerilogRight, var) => {
+  | var, m with m (TaggedVariable.VerilogLeft, var), m (TaggedVariable.VerilogRight, var) => {
     | Some smt_name1, Some smt_name2 =>
         inr (SMTLib.Term_Eq (SMTLib.Term_Const smt_name1) (SMTLib.Term_Const smt_name2))
     | _, _ => inl "mk_var_same"%string
@@ -45,7 +45,7 @@ Equations mk_var_same (var : Verilog.variable) (namemap : VerilogSMTBijection.t)
   }
   .
 
-Equations mk_inputs_same (inputs : list Verilog.variable) (namemap : VerilogSMTBijection.t)
+Equations mk_inputs_same (inputs : list Verilog.variable) (m : VerilogSMTBijection.t)
   : sum string SMTLib.term := {
   | [], m => inr SMTLib.Term_True
   | (var :: vars), m =>
@@ -59,9 +59,9 @@ Equations mk_inputs_same (inputs : list Verilog.variable) (namemap : VerilogSMTB
       end
   }.
 
-Equations mk_var_distinct (var : Verilog.variable) (namemap : VerilogSMTBijection.t)
+Equations mk_var_distinct (var : Verilog.variable) (m : VerilogSMTBijection.t)
   : sum string SMTLib.term := {
-  | var, namemap with namemap (TaggedVariable.VerilogLeft, var), namemap (TaggedVariable.VerilogRight, var) => {
+  | var, m with m (TaggedVariable.VerilogLeft, var), m (TaggedVariable.VerilogRight, var) => {
     | Some smt_name1, Some smt_name2 =>
         inr (SMTLib.Term_Not (SMTLib.Term_Eq (SMTLib.Term_Const smt_name1) (SMTLib.Term_Const smt_name2)))
     | _, _ => inl "mk_var_distinct"%string
@@ -69,7 +69,7 @@ Equations mk_var_distinct (var : Verilog.variable) (namemap : VerilogSMTBijectio
   }
   .
 
-Equations mk_outputs_distinct (inputs : list Verilog.variable) (namemap : VerilogSMTBijection.t)
+Equations mk_outputs_distinct (inputs : list Verilog.variable) (m : VerilogSMTBijection.t)
   : sum string SMTLib.term := {
   | [], m => inr SMTLib.Term_False
   | (var :: vars), m =>
@@ -109,20 +109,17 @@ Equations mk_outputs_distinct (inputs : list Verilog.variable) (namemap : Verilo
     firstorder.
   Qed.
 
-Program Definition equivalence_query_canonical
-  (canonical_verilog1 canonical_verilog2 : Verilog.vmodule)
-  : sum string (SMT.smt_with_namemap) :=
+Program Definition equivalence_query (verilog1 verilog2 : Verilog.vmodule) : sum string (SMT.smt_with_namemap) :=
+  inputs_ok1 <- assert_dec (Verilog.module_inputs verilog1 = Verilog.module_inputs verilog2) "Inputs don't match" ;;
+  outputs_ok1 <- assert_dec (Verilog.module_outputs verilog1 = Verilog.module_outputs verilog2) "Outputs don't match" ;;
 
-  inputs_ok1 <- assert_dec (Verilog.module_inputs canonical_verilog1 = Verilog.module_inputs canonical_verilog2) "Inputs don't match" ;;
-  outputs_ok1 <- assert_dec (Verilog.module_outputs canonical_verilog1 = Verilog.module_outputs canonical_verilog2) "Outputs don't match" ;;
-
-  smt1 <- VerilogToSMT.verilog_to_smt TaggedVariable.VerilogLeft 0 canonical_verilog1 ;;
-  smt2 <- VerilogToSMT.verilog_to_smt TaggedVariable.VerilogRight (1 + SMT.max_var (SMT.query smt1)) canonical_verilog2 ;;
+  smt1 <- VerilogToSMT.verilog_to_smt TaggedVariable.VerilogLeft 0 verilog1 ;;
+  smt2 <- VerilogToSMT.verilog_to_smt TaggedVariable.VerilogRight (1 + SMT.max_var (SMT.query smt1)) verilog2 ;;
 
   let nameMap := VerilogSMTBijection.combine (SMT.nameMap smt1) (SMT.nameMap smt2) _ _ in
 
-  inputs_same <- mk_inputs_same (Verilog.module_inputs canonical_verilog1) nameMap ;;
-  outputs_distinct <- mk_outputs_distinct (Verilog.module_outputs canonical_verilog1) nameMap ;;
+  inputs_same <- mk_inputs_same (Verilog.module_inputs verilog1) nameMap ;;
+  outputs_distinct <- mk_outputs_distinct (Verilog.module_outputs verilog1) nameMap ;;
 
   prf1 <- assert_dec _ "Unknown variables in inputs_same assertion" ;;
   prf2 <- assert_dec _ "Unknown variables in outputs_distinct assertion" ;;
@@ -140,13 +137,3 @@ Program Definition equivalence_query_canonical
 .
 Next Obligation. (* No shared verilog names *) Admitted.
 Next Obligation. (* No shared SMT names *) Admitted.
-
-Definition equivalence_query (verilog1 verilog2 : Verilog.vmodule) : sum string SMT.smt_with_namemap :=
-  VerilogTypecheck.tc_vmodule verilog1 ;;
-  VerilogTypecheck.tc_vmodule verilog2 ;;
-
-  canonical_verilog1 <- VerilogCanonicalize.canonicalize_verilog verilog1 ;;
-  canonical_verilog2 <- VerilogCanonicalize.canonicalize_verilog verilog2 ;;
-
-  equivalence_query_canonical canonical_verilog1 canonical_verilog2
-.
